eve/Src/framework/eiffel2boogie/translation/e2b_options.e
@@ -18,11 +18,11 @@ feature {NONE} -- Initialization
 		do
 			is_reverification_with_inlining_enabled := False
 			is_inlining_enabled := True
-			is_automatic_inlining_enabled := True
+			is_automatic_inlining_enabled := False
 			is_automatic_loop_unrolling_enabled := False
 			is_sound_loop_unrolling_enabled := True
 			is_precondition_predicate_enabled := False
-			is_postcondition_predicate_enabled := True
+			is_postcondition_predicate_enabled := False
 			is_checking_overflow := False
 			is_checking_frame := True
 		end
